Weidenbach_Book/IsaSAT/IsaSAT_Inprocessing_LLVM.thy
@@ -607,7 +607,13 @@ sepref_def isa_deduplicate_binary_clauses_code
   supply [[goals_limit=1]]
   by sepref
 
-term units_since_last_GC_st_code
+sepref_def isa_pure_literal_elimination_wl_code
+  is isa_pure_literal_elimination_wl
+  :: \<open>[\<lambda>S. length (get_clauses_wl_heur S) \<le> sint64_max \<and> learned_clss_count S \<le> uint64_max]\<^sub>a
+     isasat_bounded_assn\<^sup>d \<rightarrow> isasat_bounded_assn\<close>
+  unfolding isa_pure_literal_elimination_wl_def Let_def
+  by sepref
+
 experiment
 begin
  export_llvm isa_simplify_clauses_with_unit_st2_code
