Weidenbach_Book/Watched_Literals/Watched_Literals_Watch_List_Simp.thy
@@ -58,7 +58,7 @@ definition cdcl_twl_full_restart_inprocess_wl_prog where
   S' \<leftarrow> cdcl_twl_local_restart_wl_spec0 S;
   S' \<leftarrow> remove_one_annot_true_clause_imp_wl S';
   T \<leftarrow> mark_duplicated_binary_clauses_as_garbage_wl S';
-  T \<leftarrow> pure_literal_elimination_round_wl T;
+  T \<leftarrow> pure_literal_elimination_wl T;
   T \<leftarrow> simplify_clauses_with_units_st_wl T;
   if get_conflict_wl T \<noteq> None then do {
     ASSERT(cdcl_twl_full_restart_wl_GC_prog_post_confl S T);
@@ -96,7 +96,7 @@ lemma cdcl_twl_full_restart_inprocess_wl_prog:
     mark_to_delete_clauses_wl_mark_to_delete_clauses_l2[THEN fref_to_Down]
     cdcl_GC_clauses_wl_cdcl_GC_clauses[THEN fref_to_Down]
     mark_duplicated_binary_clauses_as_garbage_wl
-    pure_literal_elimination_round_wl_pure_literal_elimination_round_l
+    pure_literal_elimination_wl
     simplify_clauses_with_units_st_wl_simplify_clause_with_units_st2)
   subgoal unfolding cdcl_twl_full_restart_wl_GC_prog_pre_def by blast
   subgoal by (auto dest: correct_watching'_correct_watching'_nobin)
